> Figure 3 shows a sketch of a curve $C$ and a straight line $l$.
> 
> **Given that**
> 
> - $C$ has equation $y = f(x)$ where $f(x)$ is a quadratic expression in $x$
> - $C$ cuts the $x-$axis at $0$ and $6$
> - $l$ cuts the $y-$axis at $60$ and intersects $C$ at the point $(10,80)$

$$m = \frac{80-60}{10-0}$$
$\r 2$

$y - y_1 = m(x-x_1)$
$y = 2x + 60$

$y \le 2x +60$

$(O, 6)$
$y = ax(x+6)$

$80 = a \times 10(10-6)$
$80 = 40a$
$2 = a$

$y = 2x(x-6)$
$y \me 2x(x-6)$

---

> A curve has equation $y = f(x), x \me 0$
> 
> Given that
> 
> - $f'(x) = 4x + a \sqrt x + b,$ where $\boldsymbol a$ and $\boldsymbol b$ are constants
> - the curve has a stationary point at $(4,3)$
> - the curve meets the $y-$axis at $-5$
> 
> find $f(x),$ giving your answer in simplest form.

$f'(x) = 4x + x^{1/2}a + b$

$f(x) = \frac{4x^2}{2} + \frac{ax^{3/2}}{3/2} + bx + C$

$f(x) = 2x^2 + \frac{2ax^{3/2}}{3} + bx + C$

$-5 = 2(0)^2+\frac{2a \times 0 ^{3/2}}{3} + b(0) + c$
$\r c = -5$

$f(x) = 2x^2 + \frac{2}{3}ax^{3/2} + bx - 5$

$0 = 16 + 2a + b$

$2a + b = -16$
$16 a + 12b = -72$

$a = -15, \;b = 14$

$f(x) = 2x^2 + \frac{2(-15)x^{3/2}}{3} + 14(x) -5$

$f(x) = 2x^2 -10x^{3/2} + 14x -5$

