
$$
\tan \theta = \frac{ \sin \theta }{\cos \theta}
$$

$$
\cot \theta = \frac{\cos \theta}{\sin \theta}
$$

$$
\sin \theta = \frac{1}{\csc \theta}
$$

$$
\cos \theta = \frac{1}{\sec \theta}
$$

$$
\tan \theta = \frac{1}{\cot \theta}
$$

$$
\csc \theta = \frac{1}{\sin \theta}
$$


$$
\sec \theta = \frac{1}{\cos \theta}
$$

$$
\cot \theta = \frac{1}{\tan \theta}
$$


$$
\sin ^{2} \theta + \cos ^{2} \theta = 1
$$

$$
\sec ^{2} \theta - \tan ^{2} \theta = 1
$$

$$
\csc ^{2}\theta - \cot ^{2} \theta = 1
$$

$$
\sin (-\theta) = -\sin \theta
$$

$$
\tan (-\theta) = - \tan \theta
$$

$$
\csc (- \theta ) = - \csc \theta
$$

$$
\cos (-\theta) = -\cos \theta
$$

$$
\cot (- \theta) = -\cot \theta
$$

$$
\sec ( - \theta) = \sec \theta
$$

$$
\sin \left( \frac{\pi}{2} - \theta \right) = \cos \theta
$$

$$
\tan \left(  \frac{\pi}{2} - \theta \right) = \cot \theta
$$

$$
\csc \left(  \frac{\pi}{2} - \theta \right) = \sec \theta
$$

$$
\cos \left( \frac{\pi}{2} - \theta \right) = \sin \theta 
$$

$$
\cot \left( \frac{\pi}{2} - \theta  \right) = \tan \theta
$$

$$
\sec \left(  \frac{\pi}{2} - \theta \right) = \csc \theta
$$

$$
\sin (\theta  \pm \phi) = \sin \theta \cos \phi  \pm \cos \theta \sin \phi
$$

$$
\cos ( \theta  \pm \phi) = \cos \theta \cos \phi  \mp \sin \theta \sin \phi
$$

$$
\tan (\theta  \pm \phi) = \frac{\tan \theta \pm \tan \phi}{1 + \tan \theta \tan \phi}
$$


$$
\sin ( 2\theta) = 2 \sin \theta \cos \theta
$$

$$
\cos (2\theta) = \cos ^{2} \theta - \sin ^{2} \theta
$$


$$
\cos (2\theta) = 2 \cos ^{2}\theta - 1
$$

$$
\cos (2 \theta) = 1 - 2 \sin^{2} \theta
$$

$$
\tan (2 \theta) = \frac{2\tan \theta}{1 - \tan^{2} \theta}
$$

$$
\sin^{2} \theta = \frac{1 - \cos (2\theta)}{2}
$$

$$
\cos^{2} \theta = \frac{1 + \cos (2\theta)}{2}
$$

$$
\tan^{2}\theta = \frac{1 - \cos (2\theta)}{1 + \cos (2 \theta)}
$$

$$
\sin \theta + \sin \phi = 2 \sin \left(  \frac{\theta + \phi}{2} \right) \cos \left( \frac{\theta - \phi}{2} \right)
$$

$$
\sin \theta - \sin \phi = 2 \cos \left( \frac{\theta + \phi}{2} \right) \sin \left( \frac{\theta - \phi}{2} \right)
$$

$$
\cos \theta + \cos \phi = 2 \cos \left( \frac{\theta + \phi}{2} \right) \sin \left( \frac{\theta - \phi}{2} \right)
$$

$$
\cos \theta - \cos \phi = - 2 \sin \left(  \frac{\theta + \phi}{2} \right) \sin \left( \frac{\theta - \phi}{2} \right)
$$

$$
\sin \theta \sin \phi = \frac{(\cos (\theta - \phi )-\cos (\theta + \phi))}{2}
$$

$$
\cos \theta \cos \phi = \frac{(\cos (\theta - \phi)+ \cos (\theta + \phi))}{2}
$$

$$
\sin \theta \cos \phi = \frac{(\sin (\theta + \phi)+\sin (\theta - \phi))}{2}
$$

$$
\cos \theta \sin \phi = \frac{(\sin (\theta + \phi) - \sin (\theta - \phi))}{2}
$$

