---
tags:
  - pages/refined
  - algebra
  - pure
---

$y = a(x\pm b)^2+c$

#### Worked examples

$y=x^2-6x+11$

To get $b$ (the number inside the bracket), halve the coefficient (number in front) of the second term in the original equation.

so the bracket becomes $(x-3)$

$\r y = (x-3)^2-9 + 11$
$\r y = (x-3)^2+2$

---

By completing the square, find the roots of the equation

*Completing the square:*
$y = 3x^2+12x+1$

$\r 3(x^2+4x)+1$
$\r 3((x+ 2)^2 - 4)+1$
$\r 3(x+2)^2 - 12 + 1$

$y = 3(x+2)^2 - 11$

*Substituting 0 into y to find the roots*

$y = 3(x+2)^2 - 11$

$3(x+2)^2 - 11 = 0$
$3(x+2)^2 = 11$
$(x+2)^2 = \frac{11}{3}$
$x+2 = \sqrt \frac{11}{3}$
$x = -2 \pm \sqrt \frac{11}{3}$

---

By completing the square, find the **turning point** and the equation of the **line of symmetry** of $y = x^2 + 5x - 3$

$y = (x+\frac{5}{2}x)^2-(\frac{5}{2})^2-3$
$y = (x+\frac{5}{2})^2-9.25$

*finding the roots by substituting in y as 0*

$(x+\frac{5}{2})^2-9.25 = 0$

$x+\frac{5}{2} = \sqrt {9.25}$

$x = - \frac{5}{2} \pm \sqrt {9.25}$

*finding the turning point by substituting in 0*

$y = (0+\frac{5}{2})^2-9.25$
$y = -9.25$

$(x+\frac{5}{2})^2-9.25 = -9.25$
$(x+\frac{5}{2})^2=0$
$x+ \frac{5}{2} = 0$
$x = -2.5$

the minimum point of $y = x^2 + 5x - 3$ is $\bl-2.5, -9.25\br$
the line of symmetry is $x = -2.5$

---

By completing the square, determine the turning point of the graph $y = -x^2+ 4x -5$ and therefore the number of roots.

$y = -x^2+ 4x -5$

$\r -1(x^2- 4x) -5$
$\r -1((x- 2)^2-4) -5$
$\r -(x- 2)^2-1$

$y = -(x- 2)^2-1$

*finding the turning point*

$-(x-2)^2 = 0$
$-(x-2) = 0$
$x=2$

$y = -(2-2)^2$
$y = -(0)^2$
$y = -1$

The turning point of the equation $y = -x^2+ 4x -5$ is $\bl 2, -1\br$

The maximum point is below the $x$-axis, which means there are no roots. We can prove this by substituting in $y$ as $0$

$-(x- 2)^2-1= 0$
$(x- 2)^2= -1$
$x- 2= \sqrt {-1}$
$x= 2 \pm \sqrt {-1}$

Cannot $\sqrt {-1}$
$\therefore$ No real roots

---

By completing the square, find the turning point and the equation of the line of symmetry of the quadratic function:
$y = 2x^2-8x+3$

$y = 2(x^2-8x)+3$
$y = 2((x-4)^2-16)+3$
$y = 2(x-4)^2-32+3$
$y = 2(x-4)^2-29$

*finding the $x$ axis intersects*

$2(x-4)^2-29=0$
$x=4 \pm \sqrt {\frac{29}{2}}$
$x = 7.808, 0.192$

*finding the turning point*

$y = 2(0-4)^2-29$
$y = -29$

$2(x-4)^2-29=29$
$2(x-4)^2=0$
$x-4=\sqrt 0$
$x= 4$

the equation $y = 2x^2-8x+3$ has a turning point at $(4,-29)$
the line of symmetry is at $x = 4$

---

By completing the square, find the turning point and the equation of the line of symmetry of the quadratic function:
$y = -3x^2+12x-8$

$-3(x^2+-4x)-8$
$-3((x-2)^2-4)-8$
$-3(x-2)^2+12-8$
$-3(x-2)^2+4$

$y = -3(x-2)^2+4$

*finding the turning point*

$y = -3(0-2)^2+4$
$y = 4$

$-3(x-2)^2+4 = 4$
$x = 2$

The maximum point, or turning point, of the equation $y = -3x^2+12x-8$ is at the point $(2,4)$
The line of symmetry is $x =2$

---

By completing the square, determine the turning point and the equation of the line of symmetry of the quadratic function:
$y = x^2 -6x + 9$

$(x-3)^2 -9 + 9$
$y = (x-3)^2$

*turning point*

$y = (0-3)^2$
$y = 0$

$(x-3)^2 = 0$
$x = 3$

*turning point:* $\bl 3,0\br$
*line of sym:* $x=3$

---

By completing the square, find the turning point and the equation of the line of symmetry of the quadratic function:
$y= 4x^2+16x+11$



---

By completing the square, determine the turning point and the equation of the line of symmetry of the quadratic function:
$y= -2x^2+10x-7$